LiveVerif/src/LiveVerifExamples/ring_buffer.v
@@ -1,0 +1,36 @@
+(* -*- eval: (load-file "../LiveVerif/live_verif_setup.el"); -*- *)
+Require Import LiveVerif.LiveVerifLib.
+Require Import bedrock2.RecordPredicates.
+
+Load LiveVerif.
+
+Record raw_ring_buffer_t := {
+  capacity: uint_t 32;
+  dequeue_pos: uint_t 32;
+  n_elems: uint_t 32;
+  data: array_t word capacity;
+}.
+
+Global Instance raw_ring_buffer: RepPredicate raw_ring_buffer_t := ltac:(create_predicate).
+
+Definition ring_buffer(cap: Z)(vs: list word)(addr: word): mem -> Prop :=
+  ex1 (fun b: raw_ring_buffer_t =>
+    sep (raw_ring_buffer b addr)
+        (emp (capacity b = cap /\ n_elems b = len vs /\
+             (data b ++ data b)[dequeue_pos b : dequeue_pos b + n_elems b] = vs))).
+
+#[export] Instance spec_of_ring_buf_enq: fnspec :=                              .**/
+
+void ring_buf_enq(uintptr_t b_addr, uintptr_t v) /**#
+  ghost_args := cap vs (R: mem -> Prop);
+  requires t m := <{ * ring_buffer cap vs b_addr
+                     * R }> m /\
+                  len vs < cap;
+  ensures t' m' := t' = t /\
+       <{ * ring_buffer cap (vs ++ [|v|]) b_addr
+          * R }> m' #**/                                                   /**.
+Derive ring_buf_enq SuchThat (fun_correct! ring_buf_enq) As ring_buf_enq_ok.    .**/
+{                                                                          /**.
+Abort.
+
+End LiveVerif. Comments .**/ //.
